theories/SemSound.v
@@ -5,6 +5,7 @@ From LambdaST Require Import
   Environment
   FV
   Hole
+  Derivative
   Ind
   Inert
   Nullable
@@ -34,66 +35,111 @@ Proof.
     exists p. sinvert H6. unfold singleton_env. hauto lq: on use:eqb_refl.
 Qed. *)
 
-Definition Preserves i eta p e :=
-    (MaximalOn (fv e) eta -> MaximalPrefix p)
+Definition Preserves i eta p s :=
+    (MaximalOn s eta -> MaximalPrefix p)
     /\
-    (i = Inert -> EmptyOn (fv e) eta -> EmptyPrefix p)
+    (i = Inert -> EmptyOn s eta -> EmptyPrefix p)
 .
 
-Definition P_sound G (e : term) s eta (e' : term) p :=
-  WFContext G ->
-  EnvTyped eta G ->
+Theorem preserves_to_agree : forall i eta p s S' S x,
+Subset S' S ->
+Preserves i eta p S' ->
+Agree i eta (singleton_env x p)
+  S (fv (CtxHasTy x s))
+.
+Proof.
+intros.
+unfold Preserves in *.
+unfold Agree in *.
+destruct H0 as [A B].
+split; intros.
++ assert (MaximalOn S' eta) by best use:prop_on_contains.
+  cbn. intros. exists p. destruct H2. hauto lq: on use:eqb_refl.
++ assert (EmptyOn S' eta) by best use:prop_on_contains.
+  cbn. intros. exists p. destruct H3. hauto lq: on use:eqb_refl.
+Qed.
+
+
+Definition P_sound g (e : term) s eta (e' : term) p :=
+  WFContext g ->
+  EnvTyped eta g ->
     PrefixTyped p s /\
-    Preserves Jumpy eta p e
+    (forall g' s', Derivative p s s' -> ContextDerivative eta g g' -> Typed g' e' s') /\
+    Preserves Jumpy eta p (fv e)
 .
 
-Theorem soundout : forall G e s eta e' p,
+Theorem sound : forall G e s eta e' p,
     Typed G e s ->
     Step eta e e' p ->
     P_sound G e s eta e' p.
 Proof.
-    apply (lex_ind P_sound); unfold P_sound in *; intros.
-    - admit.
-    - sauto lq: on.
-    - hauto l: on use:maps_to_has_type_reflect.
-    - sauto lq: on.
-    - eapply wf_fill_reflect in H7; [|eauto].
-      assert (H00 : PrefixTyped (PfxParPair p1 p2) (TyPar s t)) by hauto l: on use:maps_to_has_type_reflect. sinvert H00.
-      edestruct IHe as [A B]; [ eapply wf_fill_reflect; eauto; sauto | eapply parlenvtyped; eauto |]. admit. (* not possible to establish disjoint here, need weaker. *)
-      admit.
-    (* induction Hstep; intros.
-    - admit.
-    - admit.
-    - admit.
-    - sinvert Ht; admit.
-    - sinvert Hstep.
-      assert (~fv G z) by hauto q: on use:wf_fill_reflect.
-      eapply IHHt; [| | eauto].
-      + admit.
-      + admit. (*eapply catlenvtyped; eauto; sauto l: on use: maps_to_has_type.*)
-    - sinvert Hwf. sinvert Heta. sinvert Hstep.
-      + constructor. eapply IHHt1; sauto lq: on rew: off.
-      + constructor. eapply IHHt1; sauto lq: on rew: off. eauto. sauto lq: on rew: off.
-    - sinvert Hstep; eapply IHHt; [| | eauto | | | eauto].
-      + eapply hmm'_reflect; eauto.
-      + eapply catrenvtyped1; admit.
-      + eapply hmm'_reflect; eauto.
-      + assert (PrefixTyped (PfxCatBoth p1 p2) (Types.TyDot s t)) by hauto l: on use:maps_to_has_type_reflect.
-        sinvert H4.
-        eapply catrenvtyped2; eauto. 
-    - sauto lq: on.
-    - sauto lq: on.
-    - sinvert Hstep. 
-      sauto use: maps_to_has_type_reflect.
-    - sfirstorder.
-    - sinvert Hstep. 
-      assert (PrefixTyped p0 s). eapply IHHt1; eauto. sfirstorder use:maps_to_hole_reflect.
-      eapply IHHt2; [ | | eauto].
-      + eapply wf_fill_reflect. eauto. sfirstorder use:wf_fill_reflect.
-      + eapply letenvtyped; eauto.
-      admit.
-        (* eapply agree_step_inert; eauto. *)
-    - sinvert Hstep. eapply IHHt; [ | | eauto]. eapply wf_fill_reflect. eauto. sfirstorder use:wf_fill_reflect. admit. *)
+    apply (lex_ind P_sound); unfold P_sound in *; intros; admit.
+Admitted.
+
+Definition P_sound_args g_in (e : argsterm) g_out eta_in (e' : argsterm) g_out' eta_out :=
+  WFContext g_out ->
+  WFContext g_in ->
+  EnvTyped eta_in g_in ->
+    EnvTyped eta_out g_out /\
+    SetEq (dom eta_out) (fv g_out) /\
+    (Agree Jumpy eta_in eta_out (fv g_in) (fv g_out)) /\
+    (forall g_in', ContextDerivative eta_in g_in g_in' -> ArgsTyped g_in' e' g_out')
+.
+
+(* this is basically how this theorem needs to go, but we have to figure out how to tie the knot with the regular soundness theorem. *)
+Theorem soundargs : forall g_in e g_out g_out' eta_in e' eta_out,
+    ArgsTyped g_in e g_out ->
+    ArgsStep eta_in g_out e e' g_out' eta_out ->
+    P_sound_args g_in e g_out eta_in e' g_out' eta_out.
+Proof.
+  intros.
+  generalize dependent g_in.
+  induction H0; unfold P_sound_args in *; intros.
+  - best.
+  - sinvert H1. 
+    edestruct sound as [A [B C]]; eauto.
+  split; try split; try split.
+    + eapply env_typed_singleton; eauto.
+    + sfirstorder use:dom_singleton.
+    + sfirstorder use:dom_singleton.
+    + eapply preserves_to_agree; [|eauto]. sfirstorder use:typing_fv.
+    + sauto lq: on.
+  - sinvert H. sinvert H0.
+    edestruct IHArgsStep1 as [A [B [C D]]]; eauto.
+    edestruct IHArgsStep2 as [E [F [G H]]]; eauto.
+    split; try split; try split.
+    + eapply env_typed_comma; [| eauto | eauto]. hauto q: on.
+    + hauto q: on.
+    + hauto drew: off.
+    + admit.
+    + sauto lq: on rew: off.
+  - sinvert H1; sinvert H2; sinvert H4; sinvert H3.
+    edestruct IHArgsStep as [A [B [C D]]]; eauto.
+    split; try split; try split.
+    + eapply env_typed_semic; [| eauto| sfirstorder use:empty_env_for_typed | hauto lq: on use:empty_env_for_empty] . 
+      clear D; clear C; clear H13; clear H9; clear H11; clear H; clear H0; clear IHArgsStep.
+      assert (Subset (fv g3) (dom eta)) by best use:envtyped_dom.
+      assert (Subset (fv g0) (dom eta)) by best use:envtyped_dom.
+      hauto lq:on rew: off use:empty_env_for_dom.
+    + cbn. hauto q: on use:empty_env_for_dom.
+    + cbn. hauto q: on use:empty_env_for_dom.
+    + admit.
+    + intros. sinvert H1. econstructor. eauto.
+      destruct H13.
+      * assert (H00 : D' = g3) by best use:context_derivative_emp'.
+        destruct H00.
+        eauto.
+      (* contradictory. *)
+      * sfirstorder.
+  - sinvert H0. sinvert H1. sinvert H3. sinvert H2.
+    edestruct IHArgsStep1 as [A [B [C D]]]; eauto.
+    edestruct IHArgsStep2 as [E [F [G H']]]; eauto.
+    split; try split; try split.
+    + eapply env_typed_semic; [| eauto | eauto | eauto]. hauto q: on.
+    + hauto q: on.
+    + hauto drew: off.
+    + admit.
+    + sauto q: on.
 Admitted.
 
 (* let x = e in e' | *)
